pulse/share/pulse/examples/PulseExample.BubbleSort.fst
@@ -258,7 +258,7 @@ fn bubble_sort
         prefix_le_suffix (value_of a) (SZ.v vi + 1) /\
         (SZ.v !j > 0 ==> is_max_up_to (value_of a) (SZ.v !j))
       )
-    decreases (Prims.op_Minus (SZ.v vi) (SZ.v (!j)))
+    decreases (SZ.v vi - SZ.v (!j))
     {
       let vj = !j;
       
