pulse/share/pulse/examples/by-example/exercises/PulseTutorialExercises.SumArray.fst
@@ -102,7 +102,7 @@ fn compare (#t:eqtype) #p1 #p2 (a1 a2:A.array t) (l:SZ.t)
       (forall (i:nat). i < v vi ==> Seq.index 's1 i == Seq.index 's2 i)
     )
   )
-  decreases (Prims.op_Minus (v l) (v (!i)))
+  decreases (v l - v (!i))
   {
     let vi = !i; 
     i := vi + 1sz
